% \documentclass[a4paper,landscape,columns=2]{cheatsheet}
\documentclass[10pt, a4paper]{article}

\usepackage{geometry}

\input{mymathpreamble.tex}

% giving this a try:
% http://www.khirevich.com/latex/microtype/
\usepackage[activate={true,nocompatibility},final,tracking=true,kerning=true,spacing=true,factor=1100,stretch=10,shrink=10]{microtype}

\usepackage{pdflscape}

\usepackage{multicol}
\setlength{\columnsep}{0.8cm}

\usepackage{wrapfig}

\usepackage{titlesec}
\titleformat*{\section}{\large\bfseries}
\titlespacing*{\section}{0pt}{2ex}{2ex}  % 4.3ex plus .2ex

\usepackage{tabularx}
\usepackage{booktabs}
\usepackage{tcolorbox}
\usepackage{enumitem}

\usepackage{tikz}
\usepackage{tikzducks}

\usepackage[style=numeric]{biblatex}
\addbibresource{bibliography.bib}

\usepackage{hyperref}
\usepackage{cleveref}

\setcounter{secnumdepth}{0}  % get rid of section numbering - no need to use \section*

% https://tex.stackexchange.com/a/390653
\newlength{\interwordspace}
\settowidth{\interwordspace}{\ }

\pagenumbering{gobble}

\begin{document}

% \setlength{\abovedisplayskip}{0pt}
% \setlength{\belowdisplayskip}{0pt}
% \setlength{\abovedisplayshortskip}{0pt}
% \setlength{\belowdisplayshortskip}{0pt}

\newgeometry{margin=10mm}

\begin{landscape}
\begin{multicols}{2}
    \raggedcolumns

    \section{Coupled ODEs}

    \[\dot{\vec{y}} = \mat{A} \vec{y} + \vec{r}\]
    %
    \[
        \ddot y + p(t) y + q(t) = r(t) \longrightarrow
        \begin{pmatrix}
            y \\
            \dot y
        \end{pmatrix}
        = \dot{\vec{y}} = \begin{pmatrix}
            0 & 1 \\
            -q(t) & -p(t)
        \end{pmatrix} \vec{y} + \begin{pmatrix}
            0 \\
            r(t)
        \end{pmatrix}
    \]

    The eigenvalues of \(\mat{A}\) found by solving \(\det (\mat{A} - \lambda \mat{I}) = 0\)
    gives the same characteristic equation for the uncoupled system. General solutions for
    a second-order system with real constant coefficients, with
    eigenvalues \(\lambda_1, \lambda_2\) and eigenvectors \(\vec{x_1}, \vec{x_2}\), are given by:
    \begin{align*}
        \lambda_1 \neq \lambda_2: \enspace
            \vec{y} &= c_1 \vec{x_1} e^{\lambda_1 t} + c_2 \vec{x_2} e^{\lambda t} \\
        \lambda_1, \lambda_2 \in \mathbb{C}: \enspace
            \vec{y} &= c_1 \Re\left(\vec{x_1} e^{\lambda_1 t}\right) 
                + c_2 \Im\left(\vec{x_1} e^{\lambda_1 t}\right) \\
        \lambda_1 = \lambda_2: \enspace
            \vec{y} &= c_1 \vec{x} e^{\lambda t} + c_2 (t \vec{x} + \vec{p}) e^{\lambda t},
            \,\text{where}\, (\mat{A} - \lambda \mat{I}) \vec{p} = \vec{x}.
    \end{align*}

    \section{Phase Portraits of 2D Autonomous Systems}

    Let \(\dot{\vec{y}} = \vec{f}(\vec{y})\) with \(\vec{y} \in \mathbb{R}^2\),
    \(\vec{f}: \mathbb{R}^2 \to \mathbb{R}^2\), where \(\vec{f}\) does not depend on \(t\).
    \(\vec{f}\) defines a direction field in
    the \(y_1\)-\(y_2\) plane, and a trajectory of the system is a curve following the
    field. \(\vec{f}\) being continuous with continuous partials implies existence and uniqueness
    for these trajectories, so they do not cross. By the chain rule, the slope of a trajectory is
    \[\oderiv{y_2}{y_1} = \frac{\dot y_2}{\dot y_1} = \frac{f_2}{f_1}.\]

    A nullcline is a curve in phase space where the slope of the trajectory is either 0 or \(\infty\).
    Set \(\dot y_2 = 0\) for horizontal nullclines and \(\dot y_1 = 0\) for vertical nullclines, and
    solve for \(y_2\). Solving for the trajectories themselves is possible in specific cases,
    usually when the ODE in \(y_2\) from the slope formula is separable.

    For the lines in phase space in the direction of the eigenvectors (called eigendirections),
    there are straight line solutions either flowing towards or away from the origin, determined
    by the sign of the corresponding eigenvalue (\(-\) stable, \(+\) unstable).
    
    \(\lambda_1 \neq \lambda_2\) and both have the same sign:
    \begin{itemize}
        \item Negative \(\lambda\) gives a \emph{stable improper node}, where
            trajectories curve like a parabola and approach the gendirection with smallest absolute value,
            since that exponential term dominates at large \(t\).
        \item Positive \(\lambda\) gives an
            \emph{unstable improper node}, where trajectories approach eigendirection with
            largest absolute value.
    \end{itemize}

    \(\lambda_1 > 0,\, \lambda_2 < 0\):
    \begin{itemize}
        \item This gives a \emph{saddle point}. Trajectories come in parallel to the
            stable eigendirection then turn around and become parallel to the unstable direction.
    \end{itemize}
    %
    \vfill\columnbreak
    %
    \(\lambda_1 = \lambda_2\):
    \begin{itemize}
        \item If there are 2 linearly independent eigenvectors (eigenspace of \(\lambda\) has dimension 2),
            all trajectories travel in straight lines either towards or away from the origin, called
            a \emph{proper node}. For a 2D system, this is only possible if \(\mat{A}\) is some multiple of
            the identity matrix, i.e. \(\mat{A} = k \mat{I}\) for \(k \in \mathbb{R}\).
        \item If there is only 1 eigenvector, trajectories come tangent to the eigendirection near the origin
            and do a U-turn away, called a \emph{degenerate node}.
    \end{itemize}

    \(\lambda = \alpha \pm \beta i\):
    \begin{itemize}
        \item If \(\alpha = 0\), trajectories are ellipses around the origin, and the origin
            is called a \emph{centre}. To determine the direction of flow, consider the sign of \(\dot y_1\)
            at a point in the positive quadrant.
        \item If \(\alpha \neq 0\), trajectories trace out a logarithmic spiral \(r(t) = e^{\alpha t}\)
            shown by converting to polar coordinates. This is called a \emph{spiral}.
            Plotting nullclines helps with sketching trajectories.
    \end{itemize}

    The following stability chart allows for the system to be classified given values of
    \(\tr \mat{A}\) and \(\det \mat{A}\) \cite{StabilityDiagram}. The discriminant
    \(\Delta\) is defined as \(\Delta = (\tr \mat{A})^2 - 4 \det \mat{A}\).

    {%
        \centering
        \includegraphics[width=\columnwidth]{images/stabilityDiagram.png}
    }%

    \begin{tcolorbox}[colframe=red!75!black, arc=0pt, outer arc=0pt, center, hbox]
        ducky's MATH2100 summary --- \today
    \end{tcolorbox}

\end{multicols}

\pagebreak

\begin{multicols}{2}
    \section{Non-Linear or Inhomogeneous Systems}

    A system \(\dot{\vec{y}} = \vec{f}(\vec{y})\) has a critical point at \(\vec{y^*}\) if
    \(\vec{f}(\vec{y^*}) = \vec{0}\). Linear systems always have one at \(\vec{0}\), and only one
    unless \(\det \mat{A} = 0\).
    %
    An inhomogeneous linear system \(\dot{\vec{y}} = \mat{A}\vec{y} + \vec{p}\) is a linear
    translation away from a homogeneous system. Shifting the critical point at \(\vec{p}\) to
    \(\vec{0}\) via the change of variables \(\vec{x} = \vec{y} - \vec{p}\) gives the homogeneous
    \(\dot{\vec{x}} = \mat{A} \vec{x}\), so techniques discussed earlier are applicable.
    
    For a nonlinear system \(\dot{\vec{y}} = \vec{f}(\vec{y})\), the nature of the system around the
    critical point is approximated via the Jacobian matrix \(\mat{D}\vec{f}\). 
    The stability diagram can be used to classify these critical points by evaluating \(\mat{D}\vec{f}\)
    at each \(\vec{y^*}\). The linearised system near \(\vec{y^*}\) is then
    \[
        \dot{\vec{y}} = \mat{D}\vec{f} |_{\vec{y^{*}}} (\vec{y} - \vec{y^*}),
        \quad
        \mat{D}\vec{f} = \begin{pmatrix}
            \pderiv{f_1}{y_1} & \pderiv{f_1}{y_2} \\
            \pderiv{f_2}{y_1} & \pderiv{f_2}{y_2}
        \end{pmatrix}.
    \]
    %
    \section{Special Functions}

    The \emph{Dirac Delta function} \(\delta(t)\) is an ``impulse'' with infinite value at \(t = 0\) and
    zero value everywhere else, satisfying \(\int_0^{\infty} \delta(t) = 1\). \(\delta(t - a)\)
    represents an impulse at \(t = a\).

    The \emph{unit step function} \(u(t)\) is defined by
    \[
        u(t) = \begin{cases}
            0, & t < 0 \\
            1, & t \geq 0.
        \end{cases}  
    \]
    To write a piecewise-continuous function in terms of \(u\),
    if \(f(t)\) changes from \(g_1(t)\) to \(g_2(t)\) at \(t = c\), add a \(u(t-c) (g_2(t) - g_1(t))\) term
    to the new expression of \(f\) \cite{LaplacePractice}.

    The \emph{Gamma function} \(\Gamma(z)\) generalises the factorial by
    \(\Gamma(n + 1) = n!\) for \(n \in \mathbb{N}\), and is defined for all positive \(z\) by
    \[
        \Gamma(z) = \int_0^{\infty} e^{-x} x^{z-1} \,\deriv x,
    \]

    In this course the \emph{error function} is defined as
    \[
        \erf(x) = \frac{2}{\sqrt{\pi}} \int_0^x e^{-u^2} \,\deriv u.
    \]
    It is odd and monotone increasing. The following formulas may be useful for computation:
    \[
        \int_0^{\infty} e^{-u^2} \,\deriv u = \int_{-\infty}^{0} e^{-u^2} \,\deriv u
        = \frac{\sqrt{\pi}}{2},
        \quad
        \frac{1}{\sqrt{\pi}} \int_a^b e^{-u^2} \,\deriv u
        = \erf(b) - \erf(a).
    \]

    For the heat equation with parameter \(c\), the \emph{Gaussian function} \(G(x, t)\) is defined as
    \[
        G(x, t) = \frac{1}{\sqrt{4 \pi c^2 t}} \exp \left(
            \frac{-x^2}{4c^2 t}
        \right).
    \]
    \(\int_{-\infty}^{\infty} G(x, t) \,\deriv x = 1\) for \(t > 0\),
    \(\lim_{t \to 0^+} G(x, t) = 0\) for \(x \neq 0\) and
    \(\lim_{t \to 0^+} G(0, t) = +\infty\).

    \section{Laplace Transforms}

    The following formulas are given in the formula sheet for the exam, but have been
    added here for completeness.
    \[
        \laplace\{f(t)\} = F(s) = \int_0^{\infty} f(t) e^{-st} \,\deriv t
    \]

    {
    \everymath{\displaystyle}
    % \renewcommand{\arraystretch}{2}
    \begin{center}
    \begin{tabular}{cc@{\hskip 1cm}cc}
        \toprule
        \(f(t)\) & \(F(s)\) & \(f(t)\) & \(F(s)\) \\
        \midrule \\[-10pt]
        \(c\) & \(\frac{c}{s}\) & \(a g(t) + b h(t)\) & \(a G(s) + b H(s)\) \\[10pt]
        \(t^{n}\) & \(\frac{n!}{s^{n+1}}\) & \(e^{at} f(t)\) & \(F(s-a)\) \\[10pt]
        \(t^{a}\) & \(\frac{\Gamma(a+1)}{s^{a+1}}\) & \(f(t-k)u(t-k)\) & \(e^{-ks} F(s)\) \\[10pt]
        \(\cos \alpha t\) & \(\frac{s}{s^{2} + \alpha^{2}}\) & \(f'(t)\) & \(s F(s) - f(0)\) \\[10pt]
        \(\sin \alpha t\) & \(\frac{\alpha}{s^{2} + \alpha^{2}}\) & \(f''(t)\) & \(s^{2} F(s) - sf(0) - f'(0)\) \\[10pt]
        \(\delta(t - k)\) & \(e^{-ks}\) & \(t f(t)\) & \(-F'(s)\) \\[1pt]
        \bottomrule
    \end{tabular}
    \end{center}
    }

    The convolution theorem states that:
    \[
        \laplace^{-1} \left\{F(s) G(s)\right\}
        = \int_0^t f(\tau) g(t - \tau) \,\deriv \tau
        = (f * g)(t).
    \]
    If \(f(t)\) has period \(p\), then the Laplace integral can be simplified:
    \[
        \laplace\{f(t)\}
        = \frac{1}{1 - e^{-sp}} \int_0^p f(t) e^{-st} \,\deriv t.
    \]
    %
    The following formulas are not included in the formula sheet, but may be helpful to know.
    \begin{align*}
        \laplace^{-1} \left\{\frac{s}{(s^2 + \alpha^2)^2}\right\} &= \frac{1}{2\alpha} t \sin \alpha t \\
        \laplace \{f(t) u(t-k)\} &= e^{-ks} \laplace\{f(t+k)\} \tag*{\cite{LaplacePractice}} \\
        \laplace \{f^{(n)}(t)\} &= s^n F(s) - \sum_{k=1}^n s^{n-k} f^{(k-1)}(0) \\
        \laplace \{t^n f(t)\} &= (-1)^n F^{(n)}(s).
    \end{align*}

\end{multicols}


\pagebreak

% \newgeometry{left=10mm,right=10mm,top=15mm,bottom=15mm}
% \vspace*{\fill}
% \onecolumn

% \vspace{-0.5cm}
\begin{multicols}{2}
    \section{Differential Operators and Change of Variables}

    A homogeneous linear differential equation has the form \(L(u) = 0\) where \(L\) is a
    \emph{linear differential operator} satisfying \(L(u+v) = L(u) + L(v)\) and
    \(L(cu) = c L(u)\) for \(c \in \mathbb{R}\) and functions \(u, v\). This can be used
    to verify a DE is linear using the linearity of the derivative. A common differential operator
    is the del operator \(\grad\), defined in 3 dimensions by
    \(\grad = (\pderiv{}{x}, \pderiv{}{y}, \pderiv{}{z})\). It can be applied to a scalar field
    \(f\) to get \(f\)'s gradient field, or be dotted or crossed with a vector field \(\vec{v}\)
    to get its \emph{divergence} or \emph{curl}:
    \begin{gather*}
        \operatorname{grad} f = \grad f = \left(\pderiv{f}{x}, \pderiv{f}{y}, \pderiv{f}{z}\right),
        \qquad
        \div \vec{v} = \grad \cdot \vec{v} = \pfrac{v_1}{x} + \pfrac{v_2}{y} + \pfrac{v_3}{z}, \\
        \curl \vec{v} = \grad \times \vec{v} = 
        \begin{vmatrix}
            \uvec{i} & \uvec{j} & \uvec{k} \\
            \pfrac{}{x} & \pfrac{}{y} & \pfrac{}{z} \\
            v_1 & v_2 & v_3
        \end{vmatrix}.
    \end{gather*}
    Additionally, the \emph{Laplacian} is defined as \(\grad^2 = \grad \cdot \grad\). For scalar fields,
    \[
        \grad^2 f = \grad \cdot \grad f = \pderiv[2]{f}{x} + \pderiv[2]{f}{y} + \pderiv[2]{f}{z},
    \]
    and for a vector field \(\vec{v}\) in cartesian coordinates, the Laplacian is just defined
    elementwise, so \(\grad^2 \vec{v} = (\grad^2 v_1, \grad^2 v_2, \grad^2 v_3)\).
    Equivalently, it can be defined as
    \[
        \grad^2 \vec{v} = \grad(\grad \cdot \vec{v}) - \grad \times (\grad \times \vec{v}).
    \]
    The above formulas only apply for \emph{cartesian coordinates}; other coordinate systems have
    different expressions. Importantly, the Laplacian in polar coordinates is given by
    \[
        \grad^2 = \frac{1}{r} \pderiv{}{r} \left(r \pderiv{}{r}\right) + \frac{1}{r^2} \pderiv[2]{}{\theta}.
    \]
    Changing variables that a PDE is expressed in may simplify the equation and give different
    types of solutions not apparent from the initial coordinate system.
    The goal is to express derivatives in the \emph{initial} coordinates in terms of
    derivatives in the \emph{new} coordinates. If \(f(x, y)\) is changed to \(f(u, v)\) via
    \(u(x, y)\) and \(v(x, y)\), then by the chain rule,
    \begin{align*}
        \pderiv{f}{x} &= \pderiv{f}{u} \pderiv{u}{x} + \pderiv{f}{v} \pderiv{v}{x}, \\
        \pderiv{f}{y} &= \pderiv{f}{u} \pderiv{u}{y} + \pderiv{f}{v} \pderiv{v}{y}.
    \end{align*}
    Note that \(f\) can be removed from the above equations to get a relationship purely involving
    the differential operators \(\pderiv{}{x}, \pderiv{}{y}, \pderiv{}{u}\) and \(\pderiv{}{v}\).
    This can then be substituted into the original PDE to get a new equation.

    An example is with the PDE \(u_t + c u_x = 0\) for \(u(x, t)\). Changing variables to
    \(x' = x - ct\) and \(t' = t\) allows the equation to be written as \(u_{t'} = 0\), thus
    \(u(x', t') = f(x')\) and \(u(x, t) = f(x-ct)\) for differentiable \(f\). The solution is
    defined on a plane in \(x\)-\(t\) space.
    
    \section{Fourier Series}

    If a function \(f(x)\) has period \(2L\), i.e. \(f(x + 2L) = f(x)\) for all \(x\), then
    it can be written as a \emph{Fourier series}:
    \[
        f(x)
        = a_0 + \sum_{n=1}^{\infty} \left(
            a_n \cos\left(\frac{n \pi x}{L}\right)
            + b_n \sin\left(\frac{n \pi x}{L}\right)
        \right),
    \]
    with Fourier coefficients given by
    \begin{gather*}
        a_n = \frac{1}{L} \int_{-L}^{L} f(x) \cos\left(\frac{n \pi x}{L}\right) \,\deriv x,
        \quad
        b_n = \frac{1}{L} \int_{-L}^{L} f(x) \sin\left(\frac{n \pi x}{L}\right) \,\deriv x, \\
        a_0 = \frac{1}{2L} \int_{-L}^{L} f(x) \,\deriv x.
    \end{gather*}
    In the case that \(f\) is \emph{even} (\(f(-x) = f(x)\)) or \emph{odd} (\(f(-x) = -f(x)\)), the formulas for
    the coefficients can be simplified, only changing the fraction and integral bounds:
    \[
        a_0 = \frac{1}{L} \int_0^L \left(\,\cdots\right) \,\deriv x,
        \quad
        a_n = \frac{2}{L} \int_0^L \left(\,\cdots\right) \,\deriv x,
        \quad
        b_n = \frac{2}{L} \int_0^L \left(\,\cdots\right) \,\deriv x.
    \]
    Odd \(f\) makes \(a_n = 0\) for all \(n\), and even \(f\) makes \(b_n = 0\) for all \(n\).

    These simplified formulas can also be used when extending \(f\) only defined on \([0, L]\) to be
    odd or even periodic over period \(2L\). This is called a \emph{half-range expansion} of \(f\);
    odd periodic extension makes \(a_n = 0\) and even period extension makes \(b_n = 0\) for all \(n\).
    
    The following identities may be useful for computation.
    %
    \begin{align*}
        2 \sin A \sin B &= \cos(A - B) - \cos(A + B) \\
        2 \cos A \cos B &= \cos(A - B) + \cos(A + B) \\
        2 \sin A \cos B &= \sin(A - B) + \sin(A + B)
    \end{align*}
    %
    If \(f\) has period \(2L\) and is piecewise continuous within that period, then its Fourier series converges
    to \(\frac{1}{2}(f(x^{+}) + f(x^{-}))\) at every \(x\) where \(f\) has left and right derivatives.

    To derive formulas for the coefficients, define functions \(f_1\) and \(f_2\) to be orthogonal
    if \(\int_{-L}^{L} f_1(x) f_2(x) \,\deriv x = 0\). It can be shown that all functions
    \(\left\{1, \cos\left(\frac{n \pi x}{L}\right), \sin\left(\frac{n \pi x}{L}\right)\right\}\)
    are mutually orthogonal by integration by parts.
    Both sides of the Fourier Series equation can then be integrated and solved for
    the coefficients, where orthogonal terms vanish. This orthogonality is further discussed in MATH2001.

\end{multicols}

\pagebreak

\begin{multicols*}{2}

    \section{Important PDEs}

    {
    \everymath{\displaystyle}
    \begin{center}
    \begin{tabular}{cccc}
        \toprule
        Name & 1D & 2D & General \\
        \midrule
        Wave Equation & \(u_{tt} = c^2 u_{xx}\) & \(u_{tt} = c^2 (u_{xx} + u_{yy})\) & \(u_{tt} = c^2 \grad^2 u\) \\
        Heat Equation & \(u_t = c^2 u_{xx}\) & \(u_{t} = c^2 (u_{xx} + u_{yy})\) & \(u_{t} = c^2 \grad^2 u\) \\
        Laplace's Equation & \(u_{xx} = 0\) & \(u_{xx} + u_{yy} = 0\) & \(\grad^2 u = 0\) \\
        \bottomrule
    \end{tabular}
    \end{center}
    }

    These equations are all linear and homogeneous.

    \section{1D Wave, Infinite Domain}

    The general solution to the 1D wave equation \(u_{tt} = c^2 u_{xx}\) can be found with the change of
    variables \(v = x + ct\) and \(w = x - ct\), giving \(u{tt} - c^2 u_{xx} = u_{vw} = 0\).
    This results in \(u(x, t) = F(x + ct) + G(x - ct)\) for arbitrary twice-differentiable \(F, G\).

    From here, consider an infinite string with \(u(x, 0) = f(x)\) as initial deflection
    and \(u_t(x, 0) = g(x)\) as initial velocity profile. From the general solution derived earlier,
    taking derivatives gives \(u_t = c F'(x+ct) - c G'(x - ct)\) where the prime denotes a derivative with
    respect to the entire argument. After substituting initial conditions and solving for \(F\) and \(G\),
    the \emph{D'Alembert's solution} to the IVP is
    \[
        u(x, t) = \frac{1}{2}\left(f(x + ct) + f(x - ct) \right)
        + \frac{1}{2C} \int_{x - ct}^{x + ct} g(s) \,\deriv s.
    \]

    A \emph{plucked} string is modelled with \(g(x) = 0\) and \(f(x)\) arbitrary.
    A \emph{struck} string is modelled with \(f(x) = 0\) and \(g(x) = A e^{-x^2}\) for \(A \in \mathbb{R}\).
    The resulting integral can be written in terms of the error function,
    \[
        u(x, t) = B \erf(x + ct) - B \erf(x - ct),
        \quad
        B = \frac{A \sqrt{\pi}}{4c}.
    \]

    \section{1D Wave, Finite Domain}

    A finite string is modelled with \(u_{tt} - c^2 u_{xx} = 0\) on \(x \in [0, L]\) for \(t \geq 0\),
    and again has initial deflection \(u(x, 0) = f(x)\) and initial velocity profile \(u_t(x, 0) = g(x)\).
    Boundary conditions are \(u(0, t) = u(L, t) = 0\).

    By Fourier's method (discussed in a later section), the non-trivial solution to this IVP is
    \begin{align*}
        u(x, t) &= \sum_{n=1}^{\infty} \left(
            A_n \cos\left(\frac{n \pi c t}{L}\right) + B_n \sin\left(\frac{n \pi ct}{L}\right)
        \right) \sin \left(\frac{n \pi x}{L}\right) \\
        A_n &= \frac{2}{L} \int_0^L \sin\left(\frac{n \pi x}{L}\right) f(x) \,\deriv x \\
        B_n &= \frac{2}{n \pi c} \int_0^L \sin\left(\frac{n \pi x}{L}\right) g(x) \deriv x.
    \end{align*}
    Note that \(A_n\) are just the coefficients of the half-range \(\sin\) series of \(f\).

    \section{1D Heat, Finite Domain}

    Consider the 1D heat equation \(u_t = c^2 u_{xx}\) on \(x \in [0, L]\) for \(t \geq 0\),
    with ICs \(u(x, 0) = f(x)\) and BCs \(u_x(0, t) = u_x(L, t) = 0\), indicating that the endpoints
    are insulated. Again using Fourier's method, one possible solution is given by
    \(u(x, t) = A_0 \in \mathbb{R}\). A non-constant solution is given by
    \begin{align*}
        u(x, t) &= \sum_{n=0}^{\infty} A_n e^{-\left(\frac{n \pi c}{L}\right)^2 t} \cos\left(\frac{n \pi x}{L}\right) \\
        A_0 &= \frac{1}{L} \int_0^L f(x) \,\deriv x \\
        A_n &= \frac{2}{L} \int_0^L f(x) \cos\left(\frac{n \pi x}{L}\right) \,\deriv x.
    \end{align*}
    Note that \(A_n\) are just the coefficients of the half-range \(\cos\) series of \(f\).
    There is an \(\exp\) term in the series instead of \(\sin\) and \(\cos\) due to
    the first derivative \(u_t\) in the PDE.

    \section{1D Heat, Infinite Domain}

    For \(u_t = c^2 u_{xx} = 0\) on \(x \in \mathbb{R}\) for \(t \geq 0\), with IC
    \(u(x, 0) = f(x)\) and no boundary conditions, the Fourier method will not be useful. Instead,
    the Gaussian function \(G(x, t)\) is a special solution to the equation, and so is \(G(x - y, t)\)
    with \(y \in \mathbb{R}\) as a parameter. It represents an injection of 1 unit of heat energy
    at \(x = y, t = 0\). Due to the superposition principle, the following formula can be verified
    as the solution to the IVP:
    \[
        u(x, t)
        = \int_{-\infty}^{\infty} G(x - y, t) f(y) \,\deriv y
        = \frac{1}{\sqrt{4 \pi c^2 t}} \int_{-\infty}^{\infty} \exp\left(-\frac{(x-y)^2}{4c^2 t}\right) f(y) \,\deriv y.
    \]
    This is verified by distributing partial derivatives into the integral, and taing the limit as \(t \to 0\)
    to show the initial condition holds.

    \section{1D Heat, Positive Domain}

    For \(u_t = c^2 u_{xx}\) on \(x, t \geq 0\), with IC \(u(x, 0) = F(x)\) for \(x \geq 0\) and BC
    \(u(0, t) = 0\), this is converted into a problem over all of \(\mathbb{R}\) considering
    values \(x < 0\) to be \emph{unphysical} via symmetry. Define an odd extension of \(F\):
    \[
        f(x) = \begin{cases}
            F(x), & x \geq 0 \\
            -F(-x), & x < 0.
        \end{cases}
    \]
    The solution to the infinite domain problem with \(u(x, 0) = f(x)\) on \(\mathbb{R}\) is a solution to the
    original problem for \(x \geq 0\). The BC is satisfied since \(f\) odd \(\implies f(0) = 0\).
    Using such symmetric extensions is called the \emph{method of images}.
    The solution given above for the infinite case can be simplified to the following formula:
    \[
        u(x, t) = \int_0^{\infty} \left[G(x-y, t) - G(x+y, t)\right] F(y) \,\deriv y.
    \]

\end{multicols*}

\pagebreak

\begin{multicols*}{2}

    \section{1D Heat, Positive Domain (cont.)}

    For the case that an \emph{insulation condition} \(u_x(0, t) = 0\) is given instead of \(u(0, t) = 0\),
    extend \(F\) with even symmetry:
    \[
        f(x) = \begin{cases}
            F(x), & x \geq 0 \\
            F(-x), & x < 0.
        \end{cases}
    \]
    By a similar derivation as before, the solution is given by
    \[
        u(x, t) = \int_0^{\infty} \left[G(x-y, t) + G(x+y, t)\right] F(y) \,\deriv y.
    \]
    Note the \(+\) instead of \(-\) in the square brackets.

    For a non-zero boundary condition \(u(0, t) = u_0 \neq 0\), the problem can be modified
    to have the solution \(\hat u(x, t) = u(x, t) - u_0\), which also satisfies \(\hat u_t = c^2 \hat u_{xx}\)
    and has BC \(\hat u(0, t) = u(0, t) - u_0 = 0\), so the previous formulas can be used to obtain \(\hat u(x, t)\)
    using
    \[
        \hat F(x) = F(x) - u_0.
    \]
    This can then be transformed back to the original problem by adding \(u_0\) to \(\hat u(x, t)\).

    \section{1D Heat, Finite, Sinusoidal BC}

    uhh

    \section{1D Heat, Finite, Inhomogeneous, General Case}

    If there is a heat source present, the 1D heat equation is modified to \(u_t(x, t) - c^2 u_{xx}(x, t) = q(x, t)\).

\end{multicols*}

\end{landscape}

\printbibliography

\begin{figure}[b]
    \centering
    \begin{tikzpicture}[scale=0.3]
        \duck[graduate=gray!20!black,
            tassel=red!70!black]
    \end{tikzpicture} 
\end{figure}

% \vspace*{\fill}
\end{document}
